Prove wp_txnMgr__activate

src/program_proof/mvcc/mvcc_ghost.v
@@ -1,32 +1,46 @@
-From Perennial.program_proof Require Import disk_prelude.
 From iris.algebra Require Import dfrac_agree.
 From iris.algebra.lib Require Import mono_nat mono_list gmap_view.
+From Perennial.program_proof Require Import disk_prelude.
 
 Definition dbval := option u64.
 Notation Nil := (None : dbval).
 Notation Value x := (Some x : dbval).
+
+Definition N_TXN_SITES : Z := 64.
 
 (* Logical version chain. *)
 Local Definition vchainR := mono_listR (leibnizO dbval).
 Local Definition key_vchainR := gmapR u64 vchainR.
 (* GC-related ghost states. *)
 Local Definition tidsR := gmap_viewR u64 (leibnizO unit).
-Local Definition sid_tidsR := gmapR u64 (dfrac_agreeR (leibnizO (gset u64))).
+Local Definition sid_tidsR := gmapR u64 tidsR.
+Local Definition sid_min_tidR := gmapR u64 mono_natR.
+
+Local Definition sids_all := U64 <$> seqZ 0 N_TXN_SITES.
+
+Lemma sids_all_lookup (sid : u64) :
+  int.Z sid < N_TXN_SITES ->
+  sids_all !! (int.nat sid) = Some sid.
+Proof.
+  intros H.
+  unfold sids_all.
+  rewrite list_lookup_fmap.
+  rewrite lookup_seqZ_lt; last word.
+  simpl. f_equal. word.
+Qed.
 
 Class mvcc_ghostG Σ :=
   {
     mvcc_key_vchainG :> inG Σ key_vchainR;
-    mvcc_active_tidsG :> inG Σ tidsR;
-    mvcc_active_tids_siteG :> inG Σ sid_tidsR;
-    mvcc_min_tidG :> inG Σ mono_natR;
+    mvcc_sid_tidsG :> inG Σ sid_tidsR;
+    mvcc_sid_min_tidG :> inG Σ sid_min_tidR;
   }.
 
 Definition mvcc_ghostΣ :=
   #[
      GFunctor key_vchainR;
-     GFunctor tidsR;
      GFunctor sid_tidsR;
-     GFunctor mono_natR
+     GFunctor sid_min_tidR
    ].
 
 Global Instance subG_mvcc_ghostG {Σ} :
@@ -36,15 +50,12 @@ Proof. solve_inG. Qed.
 Record mvcc_names :=
   {
     mvcc_key_vchain : gname;
-    mvcc_active_tids_gn : gname;
-    mvcc_active_tids_site_gn: gname;
-    mvcc_min_tid_gn : gname
+    mvcc_sid_tids_gn : gname;
+    mvcc_sid_min_tid_gn : gname
   }.
 
 Section definitions.
-Context `{!heapGS Σ, !mvcc_ghostG Σ}.
-
-Definition mvccN := nroot .@ "mvcc_inv".
+Context `{!mvcc_ghostG Σ}.
 
 Definition vchain_ptsto γ q (k : u64) (vchain : list dbval) : iProp Σ :=
   own γ.(mvcc_key_vchain) {[k := ●ML{# q } (vchain : list (leibnizO dbval))]}.
@@ -85,43 +96,113 @@ Definition view_ptsto γ (k : u64) (v : option u64) (tid : u64) : iProp Σ :=
   ∃ vchain, vchain_lb γ k vchain ∗ ⌜vchain !! (int.nat tid) = Some v⌝.
 
 Definition mods_token γ (k tid : u64) : iProp Σ :=
-  ∃ vchain, vchain_ptsto γ (1/4) k vchain ∗ ⌜(Z.of_nat (length vchain) ≤ (int.Z tid) + 1)%Z⌝.
+  ∃ vchain, vchain_ptsto γ (1/4) k vchain ∗ ⌜Z.of_nat (length vchain) ≤ (int.Z tid) + 1⌝.
 
 Theorem view_ptsto_agree γ (k : u64) (v v' : option u64) (tid : u64) :
   view_ptsto γ k v tid -∗ view_ptsto γ k v' tid -∗ ⌜v = v'⌝.
 Admitted.
 
 (* Definitions/theorems about GC-related resources. *)
-Definition active_tids_auth γ tids : iProp Σ :=
-  own γ.(mvcc_active_tids_gn) (gmap_view_auth (DfracOwn 1) tids).
+Definition site_active_tids_half_auth γ (sid : u64) tids : iProp Σ :=
+  own γ.(mvcc_sid_tids_gn) {[sid := (gmap_view_auth (DfracOwn (1 / 2)) tids)]}.
 
-Definition active_tid γ (tid : u64) : iProp Σ :=
-  own γ.(mvcc_active_tids_gn) (gmap_view_frag (V:=leibnizO unit) tid (DfracOwn 1) tt) ∧ ⌜(int.Z tid > 0)%Z⌝.
+Definition site_active_tids_frag γ (sid : u64) tid : iProp Σ :=
+  own γ.(mvcc_sid_tids_gn) {[sid := (gmap_view_frag (V:=leibnizO unit) tid (DfracOwn 1) tt)]}.
 
-Definition active_tids_site γ (sid : u64) tids : iProp Σ :=
-  own γ.(mvcc_active_tids_site_gn) {[sid := to_dfrac_agree (DfracOwn (1/2)) tids]}.
-
-Definition min_tid_auth γ tidN : iProp Σ :=
-  own γ.(mvcc_min_tid_gn) (●MN tidN).
-
-Definition min_tid_lb γ tidN : iProp Σ :=
-  own γ.(mvcc_min_tid_gn) (◯MN tidN).
-
-Theorem active_ge_min γ (tid tidlb : u64) :
-  active_tid γ tid -∗
-  min_tid_lb γ (int.nat tidlb) -∗
-  ⌜(int.Z tidlb ≤ int.Z tid)%Z⌝.
+Lemma site_active_tids_elem_of γ (sid : u64) tids tid :
+  site_active_tids_half_auth γ sid tids -∗ site_active_tids_frag γ sid tid -∗ ⌜tid ∈ (dom (gset u64) tids)⌝.
 Admitted.
 
-Definition mvcc_invariant γ : iProp Σ :=
-  ∃ tidminN tidsactive,
-    (* TODO: owning 1/2 of logical version chains. *)
-    min_tid_auth γ tidminN ∗
-    active_tids_auth γ tidsactive ∗
-    (* TODO: tidsactive is the union of tids of each *)
-    ⌜∀ tid, tid ∈ (dom (gset u64) tidsactive) -> (int.nat tid ≥ tidminN)%nat⌝.
+Lemma site_active_tids_agree γ (sid : u64) tids tids' :
+  site_active_tids_half_auth γ sid tids -∗
+  site_active_tids_half_auth γ sid tids' -∗
+  ⌜tids = tids'⌝.
+Admitted.
 
-Definition mvcc_inv γ : iProp Σ :=
-  inv mvccN (mvcc_invariant γ).
+Lemma site_active_tids_insert {γ sid tids} tid :
+  tid ∉ dom (gset u64) tids ->
+  site_active_tids_half_auth γ sid tids -∗
+  site_active_tids_half_auth γ sid tids ==∗
+  site_active_tids_half_auth γ sid (<[tid := tt]>tids) ∗
+  site_active_tids_half_auth γ sid (<[tid := tt]>tids) ∗
+  site_active_tids_frag γ sid tid.
+Admitted.
+
+Definition active_tid γ (tid : u64) : iProp Σ :=
+  ([∨ list] sid ∈ sids_all, site_active_tids_frag γ sid tid) ∧
+  ⌜int.Z tid > 0⌝.
+
+(* Q: Can we have mono_Z? *)
+Definition site_min_tid_half_auth γ (sid : u64) tidN : iProp Σ :=
+  own γ.(mvcc_sid_min_tid_gn) {[sid := (●MN{#(1 / 2)} tidN)]}.
+
+Definition site_min_tid_lb γ (sid : u64) tidN : iProp Σ :=
+  own γ.(mvcc_sid_min_tid_gn) {[sid := (◯MN tidN)]}.
+
+Lemma site_min_tid_valid γ (sid : u64) tidN tidlbN :
+  site_min_tid_half_auth γ sid tidN -∗
+  site_min_tid_lb γ sid tidlbN -∗
+  ⌜(tidlbN ≤ tidN)%nat⌝.
+Admitted.
+
+Lemma site_min_tid_lb_weaken γ (sid : u64) tidN tidN' :
+  (tidN' ≤ tidN)%nat ->
+  site_min_tid_lb γ sid tidN -∗
+  site_min_tid_lb γ sid tidN'.
+Admitted.
+
+Lemma site_min_tid_agree γ (sid : u64) tidN tidN' :
+  site_min_tid_half_auth γ sid tidN -∗
+  site_min_tid_half_auth γ sid tidN' -∗
+  ⌜tidN = tidN'⌝.
+Admitted.
+
+Lemma site_min_tid_update {γ sid tidN tidN'} tidN'' :
+  site_min_tid_half_auth γ sid tidN -∗
+  site_min_tid_half_auth γ sid tidN' ==∗
+  site_min_tid_half_auth γ sid tidN'' ∗ site_min_tid_half_auth γ sid tidN''.
+Admitted.
+
+Definition min_tid_lb γ tidN : iProp Σ :=
+  [∗ list] sid ∈ sids_all, site_min_tid_lb γ sid tidN.
+
+Definition mvcc_inv_gc_def γ : iProp Σ :=
+  [∗ list] sid ∈ sids_all,
+    ∃ (tids : gmap u64 unit) (tidmin : u64),
+      site_active_tids_half_auth γ sid tids ∗
+      site_min_tid_half_auth γ sid (int.nat tidmin) ∗
+      ([∗ set] tid ∈ (dom (gset u64) tids), ⌜(int.nat tidmin) ≤ (int.nat tid)⌝)%nat.
+
+Theorem active_ge_min γ (tid tidlb : u64) :
+  mvcc_inv_gc_def γ -∗
+  active_tid γ tid -∗
+  min_tid_lb γ (int.nat tidlb) -∗
+  ⌜int.Z tidlb ≤ int.Z tid⌝.
+Proof.
+  iIntros "Hinv Hactive Hlb".
+  iDestruct "Hactive" as "[Hactive _]".
+  iDestruct (big_orL_exist with "Hactive") as (k sid) "[%Hlookup Htid]".
+  apply elem_of_list_lookup_2 in Hlookup.
+  iDestruct (big_sepL_elem_of with "Hlb") as "Htidlb"; first done.
+  iDestruct (big_sepL_elem_of with "Hinv") as (tids tidmin) "(Htids & Htidmin & Hle)"; first done.
+  (* Obtaining [tidmin ≤ tid]. *)
+  iDestruct (site_active_tids_elem_of with "Htids Htid") as "%Helem".
+  iDestruct (big_sepS_elem_of with "Hle") as "%Hle"; first done.
+  (* Obtaining [tidlb ≤ tidmin]. *)
+  iDestruct (site_min_tid_valid with "Htidmin Htidlb") as "%Hle'".
+  iPureIntro.
+  apply Z.le_trans with (int.Z tidmin); word.
+Qed.
 
 End definitions.
+
+Section mvccinv.
+Context `{!heapGS Σ, !mvcc_ghostG Σ}.
+
+Definition mvccN := nroot .@ "mvcc_inv".
+Definition mvccNGC := nroot .@ "mvcc_inv_gc".
+
+Definition mvcc_inv_gc γ : iProp Σ :=
+  inv mvccNGC (mvcc_inv_gc_def γ).
+
+End mvccinv.
